**April 17, 2023**

# Exercise 1.19

> There is a clever algorithm for computing the Fibonacci numbers in a logarithmic number of steps.
> Recall the transformation of the state variables _a_ and _b_ in the `fib-iter` process of section 1.2.2: _a_ <- _a_+_b_ and _b_ <- _a_.
> Call this transformation _T_, and observe that applying _T_ over and over again _n_ times, starting with 1 and 0, produces the pair Fib(_n_ + 1) and Fib(_n_).
> In other words, the Fibonacci numbers are produced by applying _T_^_n_, the _n_th power of the transformation _T_, starting with the pair (1, 0).
> Now consider _T_ to be the special case of _p_ = 0 and _q_ = 1 in a family of transformations _T_\_*p*_q_, where _T_\_*p*_q_ transforms the pair (_a_, _b_) 
> according to _a_ <- _b_*q* + _a_*q* + _a_*p* and _b_ <- _b_*p* + _a_*q*. 
>
> Show that if we apply such a transformation _T_\_*p*_q_ twice, the effect is the same as using a single transformation _T_\_*p*'*q*' of the same form, 
> and compute *p*' and *q*' in terms of *p* and *q*. 
>
> This gives us an explicit way to square these transformations, and thus we can comptute _T_^_n_ using successive squaring,
> as in the `fast-expt` procedure. Put this all toghether to complete the following procedure, which runs in a logarithmic number of steps:
```scheme
(define (fib n)
    (fib-iter 1 0 0 1 n))

(define (fib-iter a b p q count)
    (cond ((= count 0) b)
          ((even? count)
           (fib-iter a
                     b
                    (??)        ; compute p'
                    (??)        ; compute q'
                    (/ count 2)))
          (else (fib-iter (+ (* b q) (* a q) (* a p))
                          (+ (* b p) (* a q))
                          p
                          q
                          (- count 1)))))
```

## Solution

To begin understanding what's going on let's pull out the _a_ and _b_ transformations in terms of _p_ and _q_:

> _a_ <- _b_*q* + _a_*q* + _a_*p*  
> _b_ <- _b_*p* + _a_*q*

and let's also lay out the transformations, not using successive squaring, of the first couple of Fibonacci numbers, just to get a grasp on what these 
transformations are doing:

```scheme
Fib(1) (a = 1, b = 0, p = 0, q = 1, count = 1)  
a <- (* 0 1) + (* 1 1) + (* 1 0)  
b <- (* 0 0) + (* 1 1)  
b = 1  

Fib(2) (a = 1, b = 0, p = 0, q = 1, count = 2)  
a <- (* 0 1) + (* 1 1) + (* 1 0)  
b <- (* 0 0) + (* 1 1)  
Fib(1) (a = 1, b = 1, p = ?, q = ?, count = 1)  
a <- (* 1 q) + (* 1 q) + (* 1 p)   ; should equal 2  
b <- (* 1 p) + (* 1 q)             ; should equal 1  
b = 1  
; In this case p = 0 and q = 1 would satisfy this equation. p = 2 and q = 0 would satisfy a, but would not satisfy b.  

Fib(3) (a = 1, b = 0, p = 0, q = 1, count = 3)  
a <- (* 0 1) + (* 1 1) + (* 1 0)  
b <- (* 0 0) + (* 1 1)  
Fib(2) (a = 1, b = 1, p = ?, q = ?, count = 2)  
a <- (* 1 p) + (* 1 q) + (* 1 p)   ; should equal 2  
b <- (* 1 p) + (* 1 q)             ; should equal 1  
Fib(1) (a = 2, b = 1, p = ?, q = ?, count = 1)  
a <- (* 1 q) + (* 2 q) + (* 1 p)   ; should equal 3  
b <- (* 1 p) + (* 2 q)             ; should equal 2  
b = 2  
; Again, in this case p = 0 and q = 1 would satisfy this equation.
```

So turns out I'm stupid. What I've observed here is exactly what's laid out in the description:

> Now consider _T_ to be the special case of _p_ = 0 and _q_ = 1 in a family of transformations _T_\_*p*_q_, where _T_\_*p*_q_ transforms the pair (_a_, _b_) 
> according to _a_ <- _b_*q* + _a_*q* + _a_*p* and _b_ <- _b_*p* + _a_*q*. 

The part that we're supposed to be figuring out is right after this:

> Show that if we apply such a transformation _T_\_*p*_q_ twice, the effect is the same as using a single transformation _T_\_*p*'*q*' of the same form, 
> and compute *p*' and *q*' in terms of *p* and *q*. 

So what we actually want to figure out is how do we calculate _p_' and _q_' in such a way that _a_ <- 1\*_q_' + 1\*_q_' + 1\*_p_' = 3 and _b_ = 1\*_p_' + 1\*_q_' = 2.  
These values are retrieved from calculating Fib(3), where the first iteration would setup _a_ and _b_ to be equal to 1 and 1, the second iteration would
calculate _p_' and _q_', and the third iteration would be applying _p_' and _q_' to _a_ and _b_, where _b_ is our answer, which would be 2.

Well, based on this example it's pretty clear that the answer is _p_' = 1 and 1 _q_' = 1.

### Memories

> TL;DR - this section ends up being built on incorrect assertions and is not correct. Skip to [this section](#back-to-the-drawing-board) where we get back on track.

Something I just remembered from the last time we were working on a successive squaring procedure is that the `else` condition is going to be called at most twice:
once during the first iteration if _count_ is odd to begin with, and once during the last iteration when _count_ = 1.

We can use this property of the procedure to declare that when we fall into our else case the pair (_a_, _b_) will either be (1, 0) or (1, 1), for the first iteration and last iteration respectively.

Something else we know for sure is that during our first iteration, if _count_ is odd then _p_ and _q_ will be equal to 0 and 1 repectively, which takes care of our first iteration.

Using these two properties we can say that the following is true of our last (or second to last) iteration:
- If _count_ is even then our last iteration will calculate _a_ and _b_ as _a_ = 0\*_q_' + 1\*_q_' + 1\*_p_' and _b_ = 0\*_p_' + 1\*_q_'  
- If _count_ is odd then our last iteration will calculate _a_ and _b_ as _a_ = 1\*_q_' + 1\*_q_' + 1\*_p_' and _b_ = 1\*_p_' + 1\*_q_'  


If we take these two statements as truth then we can calculate the values for _p_' and _q_' for known Fibonacci numbers.

### Even Fibonacci numbers

Using the statement that we just declared that if _count_ is even then _a_ = 0\*_q_' + 1\*_q_' + 1\*_p_' and _b_ = 0\*_p_' + 1\*_q_' for our last iteration, where _b_ is our answer, 
let's take some known even Fibonacci numbers and calculate the final values of _q_' and _p_'.

```scheme
Fib(6) (a = 13, b = 8)
a = 1*q' + 1*p'
b = 1*q'
; Let's plug in our expected values
13 = q' + p'
8 = q'
; Looks like we already have our value for q', which we can use to solve for p'
q' = 8
p' = 5


; Let's take this a bit further
Fib(8) (a = 55, b = 34)
55 = q' + p'
34 = q'

q' = 34
p' = 21
```

Based on these observations it looks like _p_' will always be equal to Fib(_n_ - 1), and _q_' will always be equal to Fib(_n_), our answer.

### Odd Fibonacci numbers

Let's see if the odd Fibonacci numbers shed any light on how to calculate _p_' and _q_' in terms of _p_ and _q_.

To state again, if _count_ is odd then our last iteration will calculate _a_ and _b_ as _a_ = 1\*_q_' + 1\*_q_' + 1\*_p_' and _b_ = 1\*_p_' + 1\*_q_'.

```scheme
Fib(5) (a = 8, b = 5)
a = 1*q' + 1*q' + 1*p'
b = 1*p' + 1*q'
; Plug in our values
8 = 2*q' + p'
5 = p' + q'
; solve for p'
p' = 5 - q'
; plug into the other equation
8 = 2*q' + (5 - q')
8 = 5 + q'
q' = 3
; use this value to solve again for p'
p' = 5 - q'
p' = 2

; Thinking about these values in terms of Fib(n) it looks like q' = Fib(n - 1) and p' = Fib(n - 2)
; Let's see if this holds up for another value of n.

Fib(9) (a = 89, b = 55)
a = 2*q' + p'
b = p' + q'
; plug in Fib(n - 1) and Fib(n - 2) for p' and q' respectively
a = 2*34 + 21
b = 34 + 21
; Simplify
a = 89
b = 55
; Appears that results match!
```

### All together now

Now let's take our observations from the previous two sections to consolidate into a single calculation in terms of _p_ and _q_.

We know that if _count_ is even then _p_' = Fib(_n_ - 1) and _q_' = Fib(_n_).  
We also know that if _count_ is odd then _p_' = Fib(_n_ - 2) and _q_' = Fib(_n_ - 1).

If we look back at the initial values that are sent to `fib-iter` back in our procedures _p_ is initialized to 0 and _q_ is initialized to 1, which is the inverse of _a_ and _b_.

Therefore we should be able to calculate _p_' and _q_' using the same formula as the standard way of calculating _a_ and _b_ in a Fibonacci sequence: _a_ <- _a_ + _b_ and _b_ <- _a_. 
The only adjustment we'll need to make is to account for successive squaring.

To start we can fill in the values when not using successive squaring:
```scheme
(define (fib n)
    (fib-iter 1 0 0 1 n))

(define (fib-iter a b p q count)
    (cond ((= count 0) b)
          ((even? count)
           (fib-iter a
                     b
                     q          ; p'
                     (+ q p)    ; q'
                     (/ count 2)))
          (else (fib-iter (+ (* b q) (* a q) (* a p))
                          (+ (* b p) (* a q))
                          p
                          q
                          (- count 1)))))
(define (even? n)
    (= (remainder n 2) 0))
```

The issue here is that we're not squaring when calculating our values for _p_' and _q_', which causes them to lag behind the current value of _count_ in each iteration.

To figure this out let's take an example with actual values and observe the required transformations.

```scheme
(fib 4)
(fib-iter 1 0 0 1 4)
(fib-iter 1 0 ? ? 2) 
(fib-iter 1 0 2 3 1) ; p' must equal Fib(n - 1) and q' must equal Fib(n)
(fib-iter 5 3 2 3 0)
3


(fib 6)
(fib-iter 1 0 0 1 6)
(fib-iter 1 0 ? ? 3) ; <- shit, looks like I was wrong...
(fib-iter ? ? ? ? 2) 
(fib-iter ? ? ? ? 1)
(fib-iter 13 8 5 8 0)
9
```

### Wrong

After layout out some examples above it looks like I was wrong in my assertion that the `else` case would only be called at most twice! For example, 
Fib(14) would call it three times, once when it hits 7, again when we hit 3, and again when we hit 1.

## Back to the drawing board

Starting from scratch, we know that because this problem will require us to use successive squaring we will need to calculate _p_' and _q_' by squaring _p_ and/or _q_.
Also, the problem states that we will calculate _p_' and _q'_ in terms of _p_ and _q_, so that means that the next values will be calculated using the current values.

Let's start with an extremely simple example, and work our way up:
```scheme
(fib 2)
(fib-iter 1 0 0 1 2)
(fib-iter 1 0 ? 1 1)
(fib-iter ? 1 ? 1 0)
1
```

I've just got a feeling that _q_' is going to be calulated as `(+ (square q) p)`, and _p_' is just going to equal _q_. This equation works for the last example; let's try it for some more!

```scheme
(fib 4)
(fib-iter 1 0 0 1 4)
(fib-iter 1 0 1 1 2) ; calculate q' = (+ (square q) p) and p' = q
(fib-iter 1 0 1 2 1) ; calculate q' = (+ (square q) p) and p' = q
(fib-iter ? 3 ? ? 0)
3
```

Okay, this does not work for this example. In this example we need _q_ = 3 when _count_ = 1. Just as a shot in the dark, it looks like _q_' = `(- (* q 2) p)` and _p_' = _q_ would fulfill this function.

```scheme
(fib 4)
(fib-iter 1 0 0 1 4)
(fib-iter 1 0 1 2 2) ; calculate q' = (- (* q 2) p) and p' = q
(fib-iter 1 0 2 3 1) ; calculate q' = (- (* q 2) p) and p' = q
(fib-iter ? 3 2 3 0)
3

; let's try it for another number
(fib 8)
(fib-iter 1 0 0 1 8)
(fib-iter 1 0 1 2 4) ; calculate q' = (- (* q 2) p) and p' = q
(fib-iter 1 0 2 3 2) ; calculate q' = (- (* q 2) p) and p' = q
(fib-iter 1 0 3 4 1) ; calculate q' = (- (* q 2) p) and p' = q
(fib-iter ? 34 3 4 0) ; b = (+ (* b p) (* a q)) = (+ 0 4) = 4 !!WRONG!!
34
```

Okay, again, we have a function that doesn't work. If we stick with `(fib 8)`, though, we can try to work through this problem backwards. 
We know that during our last iteration (_count_ = 1) _q_' must equal 34, because in this scenario that is what will be required to set _b_ to 34, which is the correct answer.

```scheme
34
(fib-iter ? 34 ? 34 0)
(fib-iter 1 0 ? 34 1) ; here we know that q' must equal 34, because that is what b will be set to in the next iteration.
(fib-iter 1 0 ? ? 2)
(fib-iter 1 0 ? ? 4)
(fib-iter 1 0 0 1 8)
(fib 8)
```

## The Actual Soluction

Turns out I've way overcomplicated this, and the solution is actually fairly easy.

We can figure out the answer by simply plugging in the values for the transformation twice.

For example, we can plug in the values of the first transformation by defining _a_' and _b_' as follows:
```
a' = bq + aq + ap = (p + q)a + bq
b' = bp + aq
```

And then define _a_'' and _b_'' by applying the transformation again:
```
a'' = qb' + qa' + pa' 
    = q(bp + aq) + q(bq + aq + ap) + p(bq + aq + ap)
    = bpq + aq^2 + bq^2 + aq^2 + apq + bpq + apq + ap^2
    = (pq + q^2 + pq)b + (q^2 + q^2 + pq + pq + p^2)a
    = (2pq + q^2)b + (2q^2 + 2pq + p^2)a
b'' = pb' + qa' = p(bp + aq) + q((p + q)a + bq) = bp^2 + aqp + (p + q)aq + bq^2 = (p^2 + q^2)b + (2qp + q^2)a
```

and we can translate these expansions directly into scheme
```scheme
(define (fib n)
    (fib-iter 1 0 0 1 n))

(define (fib-iter a b p q count)
    (cond ((= count 0) b)
          ((even? count)
           (fib-iter a
                     b
                     (+ (square p) (square q))
                     (+ (* 2 p q) (square q))
                     (/ count 2)))
          (else (fib-iter (+ (* b q) (* a q) (* a p))
                          (+ (* b p) (* a q))
                          p
                          q
                          (- count 1)))))
```

I'll be honest, I'm not 100% sure how these values are extracted from the above expansion, but I almost get it.

See the [actual answer](http://community.schemewiki.org/?sicp-ex-1.19) here for more details, and a better description.

